---
title: Stewart Series Testing
---
The following problems are drawn directly from p781 of the official textbook by J. Stewart.
They are for optional, additional practice only.
They are not necessarily representative of problems on APMA 1110 exams.

Two similar-looking series are given. Test each one for convergence or divergence:
(1)
(a) $\displaystyle\sum_{n=1}^{\infty} \frac{1}{5^n}$ $\qquad$ (b) $\displaystyle \sum_{n=1}^{\infty} \frac{1}{5^n+n}$

(2)
(a) $\displaystyle \sum_{n=1}^{\infty} \frac{(-1)^n}{n^{3 / 2}}$ $\qquad$ (b) $\displaystyle \sum_{n=1}^{\infty} \frac{1}{n^{3 / 2}}$

(3)
(a) $\displaystyle \sum_{n=1}^{\infty} \frac{n}{3^n}$ $\qquad$ (b) $\displaystyle \sum_{n=1}^{\infty} \frac{3^n}{n}$

(4)
(a) $\displaystyle \sum_{n=1}^{\infty} \frac{n+1}{n}$ $\qquad$ (b) $\displaystyle \sum_{n=1}^{\infty}(-1)^n \frac{n+1}{n}$

(5)
(a) $\displaystyle \sum_{n=1}^{\infty} \frac{n}{n^2+1}$ $\qquad$ (b) $\displaystyle \sum_{n=1}^{\infty}\left(\frac{n}{n^2+1}\right)^n$

(6)
(a) $\displaystyle \sum_{n=1}^{\infty} \frac{\ln n}{n}$ $\qquad$ (b) $\displaystyle \sum_{n=10}^{\infty} \frac{1}{n \ln n}$

(7)
(a) $\displaystyle \sum_{n=1}^{\infty} \frac{1}{n+n!}$ $\qquad$ (b) $\displaystyle \sum_{n=1}^{\infty}\left(\frac{1}{n}+\frac{1}{n!}\right)$

(8)
(a) $\displaystyle \sum_{n=1}^{\infty} \frac{1}{\sqrt{n^2+1}}$ $\qquad$ (b) $\displaystyle \sum_{n=1}^{\infty} \frac{1}{n \sqrt{n^2+1}}$


Test the series for convergence or divergence:

(9) $\displaystyle\sum_{n=1}^{\infty} \frac{n^2-1}{n^3+1}$ $\qquad$ (10) $\displaystyle\sum_{n=1}^{\infty} \frac{n-1}{n^3+1}$ $\qquad$ (11) $\displaystyle\sum_{n=1}^{\infty}(-1)^n \frac{n^2-1}{n^3+1}$

(12) $\displaystyle\sum_{n=1}^{\infty}(-1)^n \frac{n^2-1}{n^2+1}$ $\qquad$ (13) $\displaystyle\sum_{n=1}^{\infty} \frac{e^n}{n^2}$ $\qquad$ (14) $\displaystyle\sum_{n=1}^{\infty} \frac{n^{2 n}}{(1+n)^{3 n}}$

(15) $\displaystyle\sum_{n=2}^{\infty} \frac{1}{n \sqrt{\ln n}}$ $\qquad$ (16) $\displaystyle\sum_{n=1}^{\infty}(-1)^{n-1} \frac{n^4}{4^n}$ $\qquad$ (17) $\displaystyle\sum_{n=0}^{\infty}(-1)^n \frac{\pi^{2 n}}{(2 n)!}$

(18) $\displaystyle\sum_{n=1}^{\infty} n^2 e^{-n^3}$ $\qquad$ (19) $\displaystyle\sum_{n=1}^{\infty}\left(\frac{1}{n^3}+\frac{1}{3^n}\right)$ $\qquad$ (20) $\displaystyle\sum_{k=1}^{\infty} \frac{1}{k \sqrt{k^2+1}}$

(21) $\displaystyle\sum_{n=1}^{\infty} \frac{3^n n^2}{n!}$ $\qquad$ (22) $\displaystyle\sum_{n=1}^{\infty} \frac{\sin 2 n}{1+2^n}$ $\qquad$ (23) $\displaystyle\sum_{k=1}^{\infty} \frac{2^{k-1} 3^{k+1}}{k^k}$

(24) $\displaystyle\sum_{n=1}^{\infty} \frac{\sqrt{n^4+1}}{n^3+n}$ $\qquad$ (25) $\displaystyle\sum_{n=1}^{\infty} \frac{1 \cdot 3 \cdot 5 \cdots \cdot(2 n-1)}{2 \cdot 5 \cdot 8 \cdots \cdot(3 n-1)}$ $\qquad$ (26) $\displaystyle\sum_{n=2}^{\infty} \frac{(-1)^{n-1}}{\sqrt{n}-1}$

(27) $\displaystyle\sum_{n=1}^{\infty}(-1)^n \frac{\ln n}{\sqrt{n}}$ $\qquad$ (28) $\displaystyle\sum_{k=1}^{\infty} \frac{\sqrt[3]{k}-1}{k(\sqrt{k}+1)}$ $\qquad$ (29) $\displaystyle\sum_{n=1}^{\infty}(-1)^n \cos \left(1 / n^2\right)$

(30) $\displaystyle\sum_{k=1}^{\infty} \frac{1}{2+\sin k}$ $\qquad$ (31) $\displaystyle\sum_{n=1}^{\infty} \tan (1 / n)$ $\qquad$ (32) $\displaystyle\sum_{n=1}^{\infty} n \sin (1 / n)$

(33) $\displaystyle\sum_{n=1}^{\infty} \frac{4-\cos n}{\sqrt{n}}$ $\qquad$ (34) $\displaystyle\sum_{n=1}^{\infty} \frac{8+(-1)^n n}{n}$ $\qquad$ (35) $\displaystyle\sum_{n=1}^{\infty} \frac{n!}{e^{n^2}}$

(36) $\displaystyle\sum_{n=1}^{\infty} \frac{n^2+1}{5^n}$ $\qquad$ (37) $\displaystyle\sum_{k=1}^{\infty} \frac{k \ln k}{(k+1)^3}$ $\qquad$ (38) $\displaystyle\sum_{n=1}^{\infty} \frac{e^{1 / n}}{n^2}$

(39) $\displaystyle\sum_{n=1}^{\infty} \frac{(-1)^n}{\cosh n}$ $\qquad$ (40) $\displaystyle\sum_{j=1}^{\infty}(-1)^j \frac{\sqrt{j}}{j+5}$ $\qquad$ (41) $\displaystyle\sum_{k=1}^{\infty} \frac{5^k}{3^k+4^k}$

(42) $\displaystyle\sum_{n=1}^{\infty} \frac{(n!)^n}{n^{4 n}}$ $\qquad$ (43) $\displaystyle\sum_{n=1}^{\infty}\left(\frac{n}{n+1}\right)^{n^2}$ $\qquad$ (44) $\displaystyle\sum_{n=1}^{\infty} \frac{1}{n+n \cos ^2 n}$

(45) $\displaystyle\sum_{n=1}^{\infty} \frac{1}{n^{1+1 / n}}$ $\qquad$ (46) $\displaystyle\sum_{n=2}^{\infty} \frac{1}{(\ln n)^{\ln n}}$ $\qquad$ (47) $\displaystyle\sum_{n=1}^{\infty}(\sqrt[n]{2}-1)^n$

(48) $\displaystyle\sum_{n=1}^{\infty}(\sqrt[n]{2}-1)$


